theories/Testing_Pre_orders/Must/Alternative_Preorder/Acceptance_Set/DefinitionAS.v
@@ -25,7 +25,7 @@
 
 From Stdlib.Unicode Require Import Utf8.
 From Stdlib.Program Require Import Equality Basics.
-From stdpp Require Import finite gmap decidable.
+From stdpp Require Import finite gmap decidable gmultiset.
 From TestingTheory Require Import ActTau gLts Bisimulation Lts_OBA Subset_Act WeakTransitions Testing_Predicate
     StateTransitionSystems InteractionBetweenLts Convergence Termination FiniteImageLTS Subset_Act.
 
@@ -33,7 +33,7 @@ From TestingTheory Require Import ActTau gLts Bisimulation Lts_OBA Subset_Act We
 
 (** ** Label abstractions *)
 
-Class AbsAction {P T FinA PreAct: Type} (A : Type) (H : ExtAction A) (gLtsP : gLts P H) (gLtsT : gLts T H) (Φ : A → FinA) (𝝳 : FinA → PreAct) :=
+Class AbsAction {P T FinA PreAct: Type} (A : Type) (H : ExtAction A) (Φ : A → FinA) (𝝳 : FinA → PreAct) {gLtsP : gLts P H} {gLtsT : gLts T H}  :=
   MkAbsAction {
     (** Client-side condition for label abstractions , Definition 5 (1) **)
     abstraction_test_spec (t : T) (μ : A) (μ' : A) : (Φ μ) = (Φ μ') -> μ ∈ (R t)-> μ' ∈ (R t);
@@ -41,20 +41,20 @@ Class AbsAction {P T FinA PreAct: Type} (A : Type) (H : ExtAction A) (gLtsP : gL
     abstraction_prog_spec (p : P) μ μ' : 𝝳 (Φ μ) = 𝝳 (Φ μ') -> (Φ μ) ∈ map_set Φ (coR p) -> (Φ μ') ∈ map_set Φ (coR p);
   }.
 
-Arguments AbsAction {_} {_} {_} {_} A H gLtsP gLtsT Φ 𝝳.
+Arguments AbsAction {_} {_} {_} {_} A H Φ 𝝳 {_} {_}.
 
 
 (** ** Finitary Label abstractions *)
 
-Class FinitaryAbsAction {FinA PreAct: Type} P T (A : Type) (H : ExtAction A) {gLtsP : gLts P H} {gLtsT : gLts T H} (Φ : A → FinA) (𝝳 : FinA → PreAct)
+Class FinitaryAbsAction P T {FinA PreAct: Type} (A : Type) (H : ExtAction A) (Φ : A → FinA) (𝝳 : FinA → PreAct) {gLtsP : gLts P H} {gLtsT : gLts T H}
   `{Countable PreAct} :=
   MkFinitaryAbsAction {
-      FinitaryAbsAction_Abs :: AbsAction A H gLtsP gLtsT Φ 𝝳;
+      FinitaryAbsAction_Abs :: @AbsAction P T FinA PreAct A H Φ 𝝳 gLtsP gLtsT;
 
       (* 𝝳 (Φ (coR p)) is a finite set, called (coR_abs p) *)
       coR_abs : P -> gset PreAct;
-      preactions_of_spec1 (p : P) (pre_μ : PreAct) : pre_μ ∈ (coR_abs p) -> pre_μ ∈ map_set (fun μ => 𝝳 (Φ μ)) (coR p);
-      preactions_of_spec2 (pre_μ : PreAct) (p : P) : pre_μ ∈ ⌈ (𝝳 ∘ Φ) ⌉ (coR p) -> pre_μ ∈ (coR_abs p);
+      coR_abs_spec1 (p : P) (pre_μ : PreAct) : pre_μ ∈ (coR_abs p) -> pre_μ ∈ ⌈ (𝝳 ∘ Φ) ⌉ (coR p);
+      coR_abs_spec2 (pre_μ : PreAct) (p : P) : pre_μ ∈ ⌈ (𝝳 ∘ Φ) ⌉ (coR p) -> pre_μ ∈ (coR_abs p);
   }.
 
 (** ** Termination condition *)
@@ -65,21 +65,159 @@ Notation "p ≼₁ q" := (bhv_pre_cond1 p q) (at level 70).
 
 (** ** Smyth preorder on acceptance sets *)
 Definition bhv_pre_cond2 `{
-  gLtsP : @gLts P A H, AbsPT : @AbsAction P T FinA PreAct A H gLtsP gLtsT Φ 𝝳,
-  gLtsQ : @gLts Q A H, AbsQT : @AbsAction Q T FinA PreAct A H gLtsQ gLtsT Φ 𝝳}
+  gLtsP : @gLts P A H, AbsPT : @AbsAction P T FinA PreAct A H Φ 𝝳P  gLtsQ gLtsT,
+  gLtsQ : @gLts Q A H, AbsQT : @AbsAction Q T FinA PreAct A H Φ 𝝳Q  gLtsQ gLtsT}
   (p : P) (q : Q) :=
   forall (s : trace A) q',
     p ⇓ s -> q ⟹[s] q' -> q' ↛ ->
-    ∃ p', p ⟹[s] p' /\ p' ↛ /\ (⌈ (𝝳 ∘ Φ) ⌉ (coR p') ⊆ ⌈ (𝝳 ∘ Φ) ⌉ (coR q')).
+    ∃ p', p ⟹[s] p' /\ p' ↛ /\ (⌈ (𝝳P ∘ Φ) ⌉ (coR p') ⊆ ⌈ (𝝳Q ∘ Φ) ⌉ (coR q')).
 
 Notation "p ≼₂ q" := (bhv_pre_cond2 p q) (at level 70).
 
 (** ** Definition of the alternative preorder *)
 Definition bhv_pre `{
-  gLtsP : @gLts P A H, AbsPT : @AbsAction P T FinA PreAct A H gLtsP gLtsT Φ 𝝳,
-  gLtsQ : @gLts Q A H, AbsQT : @AbsAction Q T FinA PreAct A H gLtsQ gLtsT Φ 𝝳}
+  gLtsP : @gLts P A H, AbsPT : @AbsAction P T FinA PreAct A H Φ 𝝳P  gLtsQ gLtsT,
+  gLtsQ : @gLts Q A H, AbsQT : @AbsAction Q T FinA PreAct A H Φ 𝝳Q  gLtsQ gLtsT}
     (p : P) (q : Q) := 
       p ≼₁ q /\ p ≼₂ q.
 
 Notation "p ≼ₐₛ q" := (bhv_pre p q) (at level 70).
+
+(* No need to define a Abstraction on toFW(L) if it is already define on L. *)
+From TestingTheory Require Import MultisetLTSConstruction ForwarderConstruction.
+
+#[global] Program Instance PreActActionForFW
+  `{@AbsAction P T FinA PreAct A H Φ 𝝳 gLtsP gLtsT}
+  `{@Prop_of_Inter P (mb A) A fw_inter H gLtsP MbgLts} 
+  : @AbsAction (P * mb A) T FinA PreAct A H Φ 𝝳 (FW_gLts gLtsP) gLtsT.
+Next Obligation.
+  intros. eapply abstraction_test_spec ;eauto.
+Qed.
+Next Obligation.
+  intros ? ? ? ? ? ? ? ? ? ? ? ? (p1, m1) μ μ' eq mem.
+  assert (Φ μ ∈ ⌈ Φ ⌉ coR (p1 ▷ m1)) as mem_h; eauto.
+  destruct mem as (μ'' & mem & eq').
+  destruct mem as (μ''' & tr' & duo & b).
+  eapply lts_refuses_spec1 in tr' as ((p , m) & tr'').
+  inversion tr'';subst.
+  - admit.
+    (* assert (Φ μ'' ∈ ⌈ Φ ⌉ coR p1) as mem.
+    { eapply map_gamma_of_action. exists μ'''. repeat split ; eauto. eapply lts_refuses_spec2 ;eauto. }
+    rewrite eq' in eq. eapply abstraction_prog_spec in eq; eauto.
+    rewrite  *)
+  - destruct (decide (non_blocking μ''')) as [nb' | b'].
+    * eapply non_blocking_action_in_ms in l; eauto. subst. admit.
+    * eapply blocking_action_in_ms in l as (eq'' & duo'' & nb''); eauto.
+      subst. eapply unique_nb in duo ; subst. contradiction.
+Admitted.
+
+#[global] Program Instance FinitaryPreActActionForFW `{CC : Countable PreAct} 
+  `{@FinitaryAbsAction P T FinA PreAct A H Φ 𝝳 gLtsP gLtsT _ _ }
+  `{@Prop_of_Inter P (mb A) A fw_inter H gLtsP MbgLts} 
+  : @FinitaryAbsAction (P * mb A) T FinA PreAct A H Φ 𝝳 (FW_gLts gLtsP) gLtsT _ _ :=
+  {| coR_abs p := coR_abs p.1 ∪ dom (gmultiset_map (fun x => 𝝳 (Φ (co x))) (mb_without_not_nb p.2));|}.
+Next Obligation.
+  intros.
+  destruct p. eapply elem_of_union in H2. destruct H2 as [in_p | in_M] ; simpl in *.
+  + eapply coR_abs_spec1 in in_p.
+    destruct in_p as (μ & mem & eq). subst.
+    exists μ. split.
+    - destruct mem as (μ' & tr & duo & b).
+      eapply lts_refuses_spec1 in tr as (p' & tr).
+      exists μ'. repeat split; eauto.
+      eapply lts_refuses_spec2. exists (p' ▷ m).
+      eapply ParLeft. exact tr.
+    - eauto.
+  + simpl in *. eapply gmultiset_elem_of_dom, elem_of_gmultiset_map in in_M.
+    destruct in_M as (μ & eq & mem).
+    exists (co μ). split; eauto.
+    exists μ. repeat split ;eauto.
+    - eapply lts_refuses_spec2.
+      assert (μ ∈ mb_without_not_nb m) as mem';eauto. 
+      eapply lts_mb_nb_with_nb_spec1 in mem as (nb & mem).
+      exists (p , m ∖ {[+ μ +]}).
+      eapply ParRight.
+      assert (m = {[+ μ  +]} ⊎ (m ∖ {[+ μ +]})) as eq''' by multiset_solver.
+      rewrite eq''' at 1.
+      eapply lts_multiset_minus. exact nb. 
+    - exact (proj2_sig (exists_dual μ)).
+    - eapply lts_mb_nb_with_nb_spec1 in mem as (nb & mem).
+      eapply dual_blocks; eauto. symmetry. exact (proj2_sig (exists_dual μ)).
+Qed.
+Next Obligation.
+  intros. destruct H2 as (μ & mem & eq). subst.
+  destruct p. destruct mem as (μ' & tr & duo & b).
+  eapply lts_refuses_spec1 in tr as ((p' , m') & eq).
+  inversion eq; subst; simpl in *.
+  + eapply elem_of_union. left.
+    eapply coR_abs_spec2.
+    exists μ. repeat split ;eauto. exists μ'. repeat split; eauto.
+    eapply lts_refuses_spec2. eauto.
+  + eapply elem_of_union. right.
+    eapply gmultiset_elem_of_dom, elem_of_gmultiset_map.
+    destruct (decide (non_blocking μ')) as [nb' | b'].
+    - exists μ'. split ;eauto.
+      * assert (μ = co μ'). { eapply unique_nb; eauto. }
+        subst. eauto.
+      * eapply non_blocking_action_in_ms in l;eauto. subst.
+        eapply lts_mb_nb_with_nb_spec2;eauto.
+        multiset_solver.
+    - assert (blocking μ') as Imp; eauto.
+      eapply blocking_action_in_ms in Imp as (mem' & duo' & nb'); eauto.
+      eapply unique_nb in duo; eauto. subst. contradiction.
+Qed.
+
+(*
+destruct H2 as (μ' & mem & eq). exists μ'. repeat split; eauto.
+Qed.
+Next Obligation.
+ intros. split.
+ - intro mem. destruct p as (p , m). destruct mem as (μ' & mem & eq).
+   destruct mem as (μ'' & tr & duo & b). eapply lts_refuses_spec1 in tr as ((p',m') & tr).
+   inversion tr; subst.
+   + eapply elem_of_union_l. simpl. eapply preactions_of_spec.
+     eapply preactions_of_fin_test_spec1. exists μ''. repeat split; eauto.
+     eapply lts_refuses_spec2; eauto.
+   + destruct (decide (non_blocking μ'')) as [nb | not_nb].
+     * assert (non_blocking μ''); eauto. eapply (non_blocking_action_in_ms m μ'' m') in nb; eauto. subst.
+       eapply elem_of_union_r. eapply gmultiset_elem_of_dom. simpl.
+       rewrite mb_union.
+       assert (gmultiset_map (λ x : A, 𝝳 (Φ (co x)))
+    (mb_without_not_nb {[+ μ'' +]} ⊎ mb_without_not_nb m') = 
+        gmultiset_map (λ x : A, 𝝳 (Φ (co x))) (mb_without_not_nb {[+ μ'' +]}) ⊎ gmultiset_map (λ x : A, 𝝳 (Φ (co x))) (mb_without_not_nb m')) as eq.
+       by eapply gmultiset_map_disj_union.
+       rewrite eq. assert ((mb_without_not_nb ({[+ μ'' +]} : gmultiset A)) = ({[+ μ'' +]} : gmultiset A)) as eq'.
+       { unfold mb_without_not_nb. assert ((elements ({[+ μ'' +]} : gmultiset A)) = [μ'']) as eq'''. rewrite gmultiset_elements_singleton. eauto.
+         unfold mb. rewrite eq'''. simpl. rewrite decide_True;eauto. multiset_solver. } unfold mb. rewrite eq'.
+       rewrite gmultiset_map_singleton.
+       assert (μ'' = (co μ')). { symmetry in duo. eapply unique_nb in duo; eauto. } subst.
+       assert (μ' = (co (co μ'))) as eq''''. { eapply dual_is_involutive. } rewrite<- eq''''. multiset_solver. 
+     * assert (blocking μ''); eauto.
+       eapply blocking_action_in_ms in not_nb as (eq & duo' & nb); eauto. subst.
+       symmetry in duo. assert (μ' = co μ'').
+       { symmetry in duo. eapply unique_nb in duo. eauto. }
+       subst. contradiction.
+ - intro mem. destruct p as (p , m). eapply elem_of_union in mem. destruct mem as [p_co_act | multiset_co_act].
+   + simpl in p_co_act. eapply preactions_of_spec in p_co_act.
+     eapply preactions_of_fin_test_spec2 in p_co_act as (μ' & mem & eq). simpl.
+     subst. exists μ'. destruct mem as (μ'' & tr & duo & b).
+     repeat split; eauto. exists μ''. repeat split; eauto. eapply lts_refuses_spec2.
+     eapply lts_refuses_spec1 in tr as (p' & tr). exists (p' ▷ m).
+     eapply ParLeft. exact tr.
+   + eapply gmultiset_elem_of_dom, elem_of_gmultiset_map in multiset_co_act. simpl in *.
+     induction m using gmultiset_ind.
+     ++ unfold mb_without_not_nb in multiset_co_act. unfold mb in multiset_co_act.
+        rewrite gmultiset_elements_empty in multiset_co_act.
+        simpl in multiset_co_act.
+        multiset_solver.
+     ++ destruct multiset_co_act as (x0 & eq & eq').
+        assert (mb_without_not_nb ({[+ x +]} ⊎ X) = mb_without_not_nb ({[+ x +]} : gmultiset A) ⊎ (mb_without_not_nb X)) as eq''''.
+        { (* rewrite mb_union. *) admit. } rewrite eq'''' in eq'.
+        eapply gmultiset_elem_of_disj_union in eq'. destruct eq' as [case1 | case2].
+        -- destruct (decide (non_blocking x)) as [nb | b].
+           ** unfold mb_without_not_nb in case1. unfold mb in case1.
+              unfold mb in case1. (* rewrite gmultiset_elements_singleton. simpl. assert (x = x0) by multiset_solver. *) admit.
+           ** (* inversion case1. *) admit.
+        -- subst. admit.
+Admitted. *)
 
